backup file with fc in progress

code/poly1305/AEAD.Poly1305_64.fst
@@ -33,8 +33,6 @@ module Spec = Spec.Chacha20Poly1305
 #reset-options "--initial_fuel 0 --max_fuel 0 --z3rlimit 100"
 
 
-#set-options "--lax"
-
 val pad_16_bytes:
   input:uint8_p ->
   len:U32.t{length input = U32.v len /\ U32.v len < 16 /\ U32.v len > 0} ->
@@ -55,9 +53,42 @@ let pad_16_bytes input len =
   Seq.lemma_eq_intro (as_seq h b) (Spec.pad_16 (as_seq h0 input));
   b
 
-
 module Poly = Hacl.Standalone.Poly1305_64
 module Impl = Hacl.Impl.Poly1305_64
+
+
+val blocks:
+  current_log:Impl.log_t ->
+  st:Impl.poly1305_state ->
+  m:Impl.uint8_p ->
+  len:U64.t{16 * U64.v len = length m} ->
+  Stack Impl.log_t
+    (requires (fun h -> Impl.(live_st h st /\ live h m /\ disjoint st.r m /\ disjoint st.h m
+      /\ red_45 (as_seq h st.h)
+      /\ red_44 (as_seq h st.r)
+    )))
+    (ensures  (fun h0 updated_log h1 -> Impl.(modifies_1 st.h h0 h1 /\ live_st h1 st /\ live_st h0 st /\ live h0 m
+      /\ red_45 (as_seq h0 st.h)
+      /\ red_44 (as_seq h0 st.r)
+      /\ red_44 (as_seq h1 st.r)
+      /\ red_45 (as_seq h1 st.h)
+      )))
+#reset-options "--initial_fuel 0 --max_fuel 0 --z3rlimit 100"
+let rec blocks log st m len =
+  let h0 = ST.get() in
+  if U64.(len =^ 0uL) then (
+    log
+  )
+  else (
+    cut (U64.v len >= 1);
+    let block = Buffer.sub m 0ul 16ul in
+    let tail  = Buffer.offset m 16ul in
+    let new_log = Impl.poly1305_update log st block in
+    let len = U64.(len -^ 1uL) in
+    blocks new_log st tail len
+  )
+
+
 
 val poly1305_alloc:
   unit -> StackInline poly1305_state
@@ -65,64 +96,260 @@ val poly1305_alloc:
     (ensures (fun h0 st h1 -> modifies_0 h0 h1 /\ live_st h1 st))
 let poly1305_alloc () = Impl.alloc ()
 
+private let lemma_div (x:nat) : Lemma (16 * (x / 16) <= x /\ 16 * (x / 16) >= 0) =
+  Math.Lemmas.lemma_div_mod x 16
+
+inline_for_extraction
+let mul_div_16 (len:U32.t) : Tot (len':U32.t{U32.v len' = 16 * (U32.v len / 16)}) =
+  lemma_div (U32.v len); Math.Lemmas.lemma_div_mod (U32.v len) 16;
+  assert_norm(pow2 4 = 16);
+  U32.(16ul *^ (len >>^ 4ul))
+
+#reset-options "--initial_fuel 0 -max_fuel 0 --z3rlimit 100"
+
+val pad_last:
+  log:log_t ->
+  st:poly1305_state ->
+  input:uint8_p{disjoint st.r input /\ disjoint st.h input} ->
+  len:U32.t{U32.v len = length input /\ U32.v len < 16} ->
+  Stack log_t
+    (requires (fun h -> live_st h st /\ live h input
+      /\ red_45 (as_seq h st.h)
+      /\ red_44 (as_seq h st.r)))
+    (ensures (fun h0 log h1 -> live_st h1 st /\ live h0 input/\ modifies_1 st.h h0 h1
+      /\ red_45 (as_seq h1 st.h)
+      /\ red_44 (as_seq h1 st.r)
+    ))
+let pad_last log st input len =
+  cut (U32.v len >= 0 /\ U32.v len < 16);
+  if U32.(len =^ 0ul) then log
+  else (
+    cut (U32.v len <> 0);
+    cut (U32.v len < 16);
+    cut (U32.v len > 0 /\ U32.v len < 16);
+    push_frame();
+    let h0 = ST.get() in
+    let b = pad_16_bytes input len in
+    let h = ST.get() in
+    let l = poly1305_update log st b in
+    pop_frame();
+    l
+  )
+
+(* val pad_last: *)
+(*   log:log_t -> *)
+(*   st:poly1305_state -> *)
+(*   input:uint8_p{disjoint st.r input /\ disjoint st.h input} -> *)
+(*   len:U32.t{U32.v len = length input /\ U32.v len < 16} -> *)
+(*   Stack log_t *)
+(*     (requires (fun h -> live_st h st /\ live h input *)
+(*       /\ red_45 (as_seq h st.h) *)
+(*       /\ red_44 (as_seq h st.r) *)
+(*         /\ (let r = as_seq h st.r in *)
+(*          let acc = as_seq h st.h in *)
+(*          let log = Ghost.reveal log in *)
+(*          invariant (Hacl.Spec.Poly1305_64.MkState r acc log)))) *)
+(*     (ensures (fun h0 log h1 -> live_st h1 st /\ live h0 input/\ modifies_1 st.h h0 h1 *)
+(*       /\ red_45 (as_seq h1 st.h) *)
+(*       /\ red_44 (as_seq h1 st.r) *)
+(*       /\ (let r' = as_seq h1 st.r in *)
+(*          let acc' = as_seq h1 st.h in *)
+(*          let log = Ghost.reveal log in *)
+(*          invariant (Hacl.Spec.Poly1305_64.MkState r' acc' log)) *)
+(*     )) *)
+(* let pad_last log st input len = *)
+(*   cut (U32.v len >= 0 /\ U32.v len < 16); *)
+(*   if U32.(len =^ 0ul) then admit() //log *)
+(*   else ( *)
+(*     cut (U32.v len <> 0); *)
+(*     cut (U32.v len < 16); *)
+(*     cut (U32.v len > 0 /\ U32.v len < 16); *)
+(*     push_frame(); *)
+(*     let h0 = ST.get() in *)
+(*     let b = pad_16_bytes input len in *)
+(*     let h = ST.get() in *)
+(*     assume (as_seq h b == Seq.slice (as_seq h b) 0 16); //Seq.lemma_eq_intro (as_seq h b) (Seq.slice (as_seq h b) 0 16); *)
+(*     Hacl.Standalone.Poly1305_64.lemma_poly1305_blocks_spec_1 (Hacl.Spec.Poly1305_64.MkState (as_seq h0 (Impl.MkState?.r st)) (as_seq h0 (Impl.MkState?.h st)) (reveal log)) (as_seq h b) 16uL; admit()) *)
+
+(*   (\*   let l = poly1305_update log st b in *\) *)
+(*   (\*   let h1 = ST.get() in *\) *)
+(*   (\*   cut (modifies_2_1 st.h h0 h1); *\) *)
+(*   (\*   pop_frame(); *\) *)
+(*   (\*   l *\) *)
+(*   (\* ) *\) *)
+
+#reset-options "--initial_fuel 0 -max_fuel 0 --z3rlimit 100"
+
 
 val poly1305_blocks_init:
   st:poly1305_state ->
   input:uint8_p{disjoint st.r input /\ disjoint st.h input} ->
   len:U32.t{U32.v len = length input} ->
   k:uint8_p{length k = 32 /\ disjoint k st.r /\ disjoint k st.h} ->
-  Stack unit
+  Stack log_t
     (requires (fun h -> live_st h st /\ live h input /\ live h k))
-    (ensures (fun h0 _ h1 -> live_st h1 st /\ live h0 input /\ live h0 k /\ modifies_2 st.r st.h h0 h1))
+    (ensures (fun h0 log h1 -> live_st h1 st /\ live h0 input /\ live h0 k /\ modifies_2 st.r st.h h0 h1
+      /\ red_45 (as_seq h1 st.h)
+      /\ red_44 (as_seq h1 st.r)
+    ))
 let poly1305_blocks_init st input len k =
-  let l = Impl.poly1305_init_ st (Buffer.sub k 0ul 16ul) in
   let len_16 = U32.(len >>^ 4ul) in
-  let rem_16 = U32.(len &^ 4ul)  in
-  let l = Poly.poly1305_blocks l st (Buffer.sub input 0ul U32.(16ul *^ len_16)) (Int.Cast.uint32_to_uint64 len_16) in
-  if U32.(rem_16 =^ 0ul) then ()
-  else (
-    push_frame();
-    let b = pad_16_bytes (Buffer.offset input U32.(len -^ rem_16)) rem_16 in
-    let _ = poly1305_update l st b in
-    pop_frame()
-  )
+  let rem_16 = U32.(len &^ 15ul)  in
+  assert_norm(pow2 4 = 16);
+  UInt.logand_mask (U32.v len) 4;
+  Math.Lemmas.lemma_div_mod (U32.v len) 16;
+  lemma_div (U32.v len);
+  let kr = Buffer.sub k 0ul 16ul in
+  let len' = mul_div_16 len in
+  let part_input = Buffer.sub input 0ul len' in
+  let last_block = Buffer.offset input len' in
+  cut (length last_block = U32.v rem_16);
+  let l = Poly.poly1305_partial st part_input (Int.Cast.uint32_to_uint64 len_16) kr in
+  pad_last l st last_block rem_16
 
 
-let fake_log : Impl.log_t = Ghost.hide (Seq.createEmpty)
+(* val poly1305_blocks_init: *)
+(*   st:poly1305_state -> *)
+(*   input:uint8_p{disjoint st.r input /\ disjoint st.h input} -> *)
+(*   len:U32.t{U32.v len = length input} -> *)
+(*   k:uint8_p{length k = 32 /\ disjoint k st.r /\ disjoint k st.h} -> *)
+(*   Stack log_t *)
+(*     (requires (fun h -> live_st h st /\ live h input /\ live h k *)
+(*     )) *)
+(*     (ensures (fun h0 log h1 -> live_st h1 st /\ live h0 input /\ live h0 k /\ modifies_2 st.r st.h h0 h1 *)
+(*       /\ red_45 (as_seq h1 st.h) *)
+(*       /\ red_44 (as_seq h1 st.r) *)
+(*       /\ (let r' = as_seq h1 st.r in *)
+(*          let acc' = as_seq h1 st.h in *)
+(*          let log = Ghost.reveal log in *)
+(*          invariant (Hacl.Spec.Poly1305_64.MkState r' acc' log)) *)
+(*     )) *)
+(* let poly1305_blocks_init st input len k = *)
+(*   let len_16 = U32.(len >>^ 4ul) in *)
+(*   let rem_16 = U32.(len &^ 15ul)  in *)
+(*   assert_norm(pow2 4 = 16); *)
+(*   UInt.logand_mask (U32.v len) 4; *)
+(*   Math.Lemmas.lemma_div_mod (U32.v len) 16; *)
+(*   lemma_div (U32.v len); *)
+(*   let kr = Buffer.sub k 0ul 16ul in *)
+(*   let len' = mul_div_16 len in *)
+(*   let part_input = Buffer.sub input 0ul len' in *)
+(*   let last_block = Buffer.offset input len' in *)
+(*   cut (length last_block = U32.v rem_16); *)
+(*   let l = Poly.poly1305_partial st part_input (Int.Cast.uint32_to_uint64 len_16) kr in *)
+(*   pad_last l st last_block rem_16 *)
 
 
 val poly1305_blocks_continue:
+  log:log_t ->
   st:poly1305_state ->
   input:uint8_p{disjoint st.h input} ->
   len:U32.t{U32.v len = length input} ->
-  Stack unit
-    (requires (fun h -> live_st h st /\ live h input))
-    (ensures (fun h0 _ h1 -> live_st h1 st /\ live h0 input /\ modifies_1 st.h h0 h1))
-let poly1305_blocks_continue st input len =
+  Stack log_t
+    (requires (fun h -> live_st h st /\ live h input
+      /\ red_45 (as_seq h st.h)
+      /\ red_44 (as_seq h st.r)
+    ))
+    (ensures (fun h0 log' h1 -> live_st h1 st /\ live h0 input /\ modifies_1 st.h h0 h1
+      /\ red_45 (as_seq h1 st.h)
+      /\ red_44 (as_seq h1 st.r)
+    ))
+let poly1305_blocks_continue log st input len =
   let len_16 = U32.(len >>^ 4ul) in
-  let rem_16 = U32.(len &^ 4ul)  in
-  let l = Poly.poly1305_blocks fake_log st (Buffer.sub input 0ul U32.(16ul *^ len_16)) (Int.Cast.uint32_to_uint64 len_16) in
-  if U32.(rem_16 =^ 0ul) then ()
-  else (
-    push_frame();
-    let b = pad_16_bytes (Buffer.offset input U32.(len -^ rem_16)) rem_16 in
-    let _ = poly1305_update l st b in
-    pop_frame()
-  )
+  let rem_16 = U32.(len &^ 15ul)  in
+  assert_norm(pow2 4 = 16);
+  UInt.logand_mask (U32.v len) 4;
+  Math.Lemmas.lemma_div_mod (U32.v len) 16;
+  lemma_div (U32.v len);
+  let len' = mul_div_16 len in
+  let part_input = Buffer.sub input 0ul len' in
+  let last_block = Buffer.offset input len' in
+  let l = blocks log st part_input (Int.Cast.uint32_to_uint64 len_16) in
+  pad_last l st last_block rem_16
 
+
+(* val poly1305_blocks_continue: *)
+(*   log:log_t -> *)
+(*   st:poly1305_state -> *)
+(*   input:uint8_p{disjoint st.h input} -> *)
+(*   len:U32.t{U32.v len = length input} -> *)
+(*   Stack log_t *)
+(*     (requires (fun h -> live_st h st /\ live h input *)
+(*       /\ red_45 (as_seq h st.h) *)
+(*       /\ red_44 (as_seq h st.r) *)
+(*       /\ (let r = as_seq h st.r in *)
+(*          let acc = as_seq h st.h in *)
+(*          let log = Ghost.reveal log in *)
+(*          invariant (Hacl.Spec.Poly1305_64.MkState r acc log)) *)
+(*     )) *)
+(*     (ensures (fun h0 log' h1 -> live_st h1 st /\ live h0 input /\ modifies_1 st.h h0 h1 *)
+(*       /\ red_45 (as_seq h1 st.h) *)
+(*       /\ red_44 (as_seq h1 st.r) *)
+(*       /\ (let r = as_seq h1 st.r in *)
+(*          let acc = as_seq h1 st.h in *)
+(*          let log' = Ghost.reveal log' in *)
+(*          invariant (Hacl.Spec.Poly1305_64.MkState r acc log')) *)
+(*     )) *)
+(* let poly1305_blocks_continue log st input len = *)
+(*   let len_16 = U32.(len >>^ 4ul) in *)
+(*   let rem_16 = U32.(len &^ 15ul)  in *)
+(*   assert_norm(pow2 4 = 16); *)
+(*   UInt.logand_mask (U32.v len) 4; *)
+(*   Math.Lemmas.lemma_div_mod (U32.v len) 16; *)
+(*   lemma_div (U32.v len); *)
+(*   let len' = mul_div_16 len in *)
+(*   let part_input = Buffer.sub input 0ul len' in *)
+(*   let last_block = Buffer.offset input len' in *)
+(*   let l = Poly.poly1305_blocks log st part_input (Int.Cast.uint32_to_uint64 len_16) in *)
+(*   pad_last l st last_block rem_16 *)
+(*   (\* if U32.(rem_16 =^ 0ul) then () *\) *)
+(*   (\* else ( *\) *)
+(*   (\*   push_frame(); *\) *)
+(*   (\*   let b = pad_16_bytes (Buffer.offset input U32.(len -^ rem_16)) rem_16 in *\) *)
+(*   (\*   let _ = poly1305_update l st b in *\) *)
+(*   (\*   pop_frame() *\) *)
+(*   (\* ) *\) *)
+
+#reset-options "--initial_fuel 0 --max_fuel 0 --z3rlimit 5"
 
 val poly1305_blocks_finish:
+  log:log_t ->
   st:poly1305_state ->
-  input:uint8_p{disjoint st.h input} ->
-  mac:uint8_p{disjoint st.h mac /\ disjoint mac input} ->
-  key_s:uint8_p{disjoint key_s st.h /\ disjoint key_s mac} ->
+  input:uint8_p{disjoint st.h input /\ length input = 16} ->
+  mac:uint8_p{disjoint st.h mac /\ disjoint mac input /\ length mac = 16} ->
+  key_s:uint8_p{disjoint key_s st.h /\ disjoint key_s mac /\ length key_s = 16} ->
   Stack unit
-    (requires (fun h -> live_st h st /\ live h input /\ live h mac))
+    (requires (fun h -> live_st h st /\ live h input /\ live h mac /\ live h key_s
+      /\ red_45 (as_seq h st.h)
+      /\ red_44 (as_seq h st.r)
+    ))
     (ensures (fun h0 _ h1 -> live h0 input /\ modifies_2 mac st.h h0 h1 /\ live h1 mac))
-let poly1305_blocks_finish st input mac key_s =
-  let _ = Impl.poly1305_update fake_log st input in
-  let _ = Impl.poly1305_update_last fake_log st (Buffer.offset input 16ul) 0uL in
+let poly1305_blocks_finish log st input mac key_s =
+  let log = Impl.poly1305_update log st input in
+  let log = Impl.poly1305_update_last log st (Buffer.offset input 16ul) 0uL in
   let _ = Impl.poly1305_finish st mac key_s in
   ()
 
 
+
+(* val poly1305_blocks_finish: *)
+(*   log:log_t -> *)
+(*   st:poly1305_state -> *)
+(*   input:uint8_p{disjoint st.h input /\ length input = 16} -> *)
+(*   mac:uint8_p{disjoint st.h mac /\ disjoint mac input} -> *)
+(*   key_s:uint8_p{disjoint key_s st.h /\ disjoint key_s mac} -> *)
+(*   Stack unit *)
+(*     (requires (fun h -> live_st h st /\ live h input /\ live h mac *)
+(*       /\ red_45 (as_seq h st.h) *)
+(*       /\ red_44 (as_seq h st.r) *)
+(*       /\ (let r = as_seq h st.r in *)
+(*          let acc = as_seq h st.h in *)
+(*          let log = Ghost.reveal log in *)
+(*          invariant (Hacl.Spec.Poly1305_64.MkState r acc log)) *)
+(*     )) *)
+(*     (ensures (fun h0 _ h1 -> live h0 input /\ modifies_2 mac st.h h0 h1 /\ live h1 mac)) *)
+(* let poly1305_blocks_finish log st input mac key_s = *)
+(*   let log = Impl.poly1305_update log st input in *)
+(*   let log = Impl.poly1305_update_last log st (Buffer.offset input 16ul) 0uL in *)
+(*   let _ = Impl.poly1305_finish st mac key_s in *)
+(*   () *)
